Fix Coq compilation issues in ThieleUniversal.v and ThieleMachineSig.v
Co-authored-by: sethirus <2708916+sethirus@users.noreply.github.com>

coq/thielemachine/coqproofs/ThieleMachineSig.v
@@ -90,12 +90,22 @@ Module MinimalThieleMachine <: THIELE_ABSTRACT.
   Definition is_LASSERT (i : Instr) : bool := TM.is_LASSERT i.
   Definition is_MDLACC (i : Instr) : bool := TM.is_MDLACC i.
 
-  Definition StepObs : Type := TM.StepObs.
+  Record StepObs := {
+    ev       : option Event;
+    mu_delta : Z;
+    cert     : Cert;
+  }.
 
   Definition mk_prog (code : list Instr) : TM.Prog := {| TM.code := code |}.
 
+  Definition to_TM_StepObs (obs : StepObs) : TM.StepObs :=
+    {| TM.ev := obs.(ev); TM.mu_delta := obs.(mu_delta); TM.cert := obs.(cert) |}.
+
+  Definition from_TM_StepObs (tm_obs : TM.StepObs) : StepObs :=
+    {| ev := tm_obs.(TM.ev); mu_delta := tm_obs.(TM.mu_delta); cert := tm_obs.(TM.cert) |}.
+
   Definition step (P : list Instr) (s s' : State) (obs : StepObs) : Prop :=
-    TM.step (mk_prog P) s s' obs.
+    TM.step (mk_prog P) s s' (to_TM_StepObs obs).
 
   Definition check_step
     (P : list Instr) (spre spost : State) (oev : option Event) (c : Cert) : bool :=
@@ -117,7 +127,10 @@ Module MinimalThieleMachine <: THIELE_ABSTRACT.
   Proof.
     intros P s s' obs Hstep.
     unfold step, check_step in *.
-    apply TM.check_step_sound.
+    destruct obs as [oev omu ocert]; simpl in *.
+    unfold to_TM_StepObs in Hstep; simpl in Hstep.
+    apply TM.check_step_sound in Hstep.
+    simpl in Hstep.
     exact Hstep.
   Qed.
 
@@ -128,7 +141,8 @@ Module MinimalThieleMachine <: THIELE_ABSTRACT.
   Proof.
     intros P s s' obs Hstep.
     unfold step, bitsize in *.
-    apply TM.mu_lower_bound.
+    simpl in *.
+    apply (TM.mu_lower_bound (mk_prog P) s s' (to_TM_StepObs obs)).
     exact Hstep.
   Qed.
 
@@ -140,8 +154,14 @@ Module MinimalThieleMachine <: THIELE_ABSTRACT.
     intros P s s' oev c Hchk.
     unfold step, check_step in *.
     apply TM.check_step_complete in Hchk.
-    destruct Hchk as [obs [Hstep [Hev Hcert]]].
-    exists obs. repeat split; assumption.
+    destruct Hchk as [tm_obs [Hstep [Hev Hcert]]].
+    exists (from_TM_StepObs tm_obs).
+    unfold from_TM_StepObs; simpl.
+    split.
+    - unfold step, to_TM_StepObs; simpl.
+      destruct tm_obs; simpl in *; subst.
+      exact Hstep.
+    - split; [exact Hev | exact Hcert].
   Qed.
 
   Lemma state_eqb_refl : forall s, state_eqb s s = true.
@@ -150,4 +170,35 @@ Module MinimalThieleMachine <: THIELE_ABSTRACT.
     unfold state_eqb.
     apply TM.state_eqb_refl.
   Qed.
+
+  (* Definitions from signature that need to be in the implementation *)
+  Definition well_formed_prog (P : list Instr) : bool :=
+    forallb (fun i => orb (is_LASSERT i) (is_MDLACC i)) P.
+
+  Definition Receipt := (State * State * option Event * Cert)%type.
+
+  Fixpoint replay_ok (P:list Instr) (s0:State) (rs:list Receipt) : bool :=
+    match rs with
+    | [] => true
+    | (spre, spost, oev, c)::tl =>
+        if negb (state_eqb spre s0) then false
+        else if check_step P spre spost oev c
+             then replay_ok P spost tl
+             else false
+    end.
+
+  Fixpoint receipts_of (P:list Instr) (s0:State)
+         (tr:list (State*StepObs)) : list Receipt :=
+    match tr with
+    | [] => []
+    | (s',obs)::tl =>
+        (s0,s',obs.(ev),obs.(cert)) :: receipts_of P s' tl
+    end.
+
+  Definition sum_mu (tr: list (State*StepObs)) : Z :=
+    fold_left (fun acc '(_,obs) => Z.add acc obs.(mu_delta)) tr 0%Z.
+
+  Definition sum_bits (rs: list Receipt) : Z :=
+    fold_left (fun acc '(_,_,_,c) => Z.add acc (bitsize c)) rs 0%Z.
+
 End MinimalThieleMachine.
